$\displaystyle f\left( x \right) = \sum\limits_{n = 0}^\infty  {\left( {n + \frac{2}{{{8^n}}}} \right){x^n}}  = \sum\limits_{n = 0}^\infty  {\left( {n{x^n} + \frac{2}{{{8^n}}}{x^n}} \right)}  = \frac{x}{{{{\left( {1 - x} \right)}^2}}} + 2\sum\limits_{n = 0}^\infty  {{{\left( {\frac{x}{8}} \right)}^n}}  = \frac{x}{{{{\left( {1 - x} \right)}^2}}} + 2\frac{1}{{1 - \frac{x}{8}}}$

$\displaystyle f\left( {\frac{1}{2}} \right) = \frac{{\frac{1}{2}}}{{{{\left( {1 - \frac{1}{2}} \right)}^2}}} + 2\frac{1}{{1 - \frac{{\frac{1}{2}}}{8}}} = \frac{{62}}{{15}}$
